Define ordered supports
Signed-off-by: zeramorphic <zeramorphic@proton.me>

ConNF/Counting/OrdSupport.lean
@@ -13,269 +13,36 @@ namespace ConNF
 variable [Params.{u}] {α : Λ} [BasePositions] [FoaAssumptions α] {β : Iic α}
 
 structure OrdSupport (β : Iic α) where
-  /-- The position of a support condition in this ordered support.
-  Named `cpos` instead of `pos` so it doesn't clash with `pos`.
-
-  The support conditions in the domain of an ordered support are well-ordered lexicographically
-  first by `cpos` then their paths. -/
-  cpos : SupportCondition β →. Atom ⊕ NearLitter
-  injective (c d : SupportCondition β) (hc : (cpos c).Dom) (hd : (cpos d).Dom) :
-    c.path = d.path → (cpos c).get hc = (cpos d).get hd → c = d
-  dom_small' : Small cpos.Dom
+  /-- The set of support conditions in this ordered support. -/
+  carrier : Set (SupportCondition β)
+  /-- An order on `carrier`. -/
+  r : carrier → carrier → Prop
+  /-- `r` is a well order. -/
+  r_isWellOrder : IsWellOrder carrier r
 
 namespace OrdSupport
 
+variable {S : OrdSupport β}
+
+instance : CoeTC (OrdSupport β) (Set (SupportCondition β)) where
+  coe := OrdSupport.carrier
+
 instance : Membership (SupportCondition β) (OrdSupport β) where
-  mem c S := (S.cpos c).Dom
+  mem c S := c ∈ S.carrier
 
-theorem mem_iff {S : OrdSupport β} {c : SupportCondition β} :
-    c ∈ S ↔ (S.cpos c).Dom :=
-  Iff.rfl
+instance : CoeSort (OrdSupport β) (Type _) :=
+  ⟨fun S => { x : SupportCondition β // x ∈ S }⟩
 
-theorem dom_small (S : OrdSupport β) : Small {c | c ∈ S} :=
-  S.dom_small'
-
-@[ext]
-theorem ext {S T : OrdSupport β}
-    (hdom : ∀ c, c ∈ S ↔ c ∈ T)
-    (h : ∀ c hcS hcT, (S.cpos c).get hcS = (T.cpos c).get hcT) :
-    S = T := by
-  rw [mk.injEq]
-  funext c
-  exact Part.ext' (hdom c) (h c)
-
-instance : MulAction (Allowable β) (OrdSupport β) where
-  smul ρ S := {
-    cpos := fun c => S.cpos (ρ⁻¹ • c)
-    injective := fun c d hc hd h₁ h₂ =>
-      smul_left_cancel _ (S.injective (ρ⁻¹ • c) (ρ⁻¹ • d) hc hd h₁ h₂)
-    dom_small' := by
-      refine lt_of_le_of_lt ?_ S.dom_small
-      refine ⟨⟨fun c => ⟨ρ⁻¹ • c.1, c.2⟩, ?_⟩⟩
-      rintro ⟨c, hc⟩ ⟨d, hd⟩
-      simp only [Subtype.mk.injEq, smul_left_cancel_iff, PFun.dom_mk, coe_setOf, mem_setOf_eq,
-        imp_self]
-  }
-  one_smul S := by
-    ext c hc₁ hc₂
-    · change (S.cpos _).Dom ↔ (S.cpos _).Dom
-      simp only [inv_one, one_smul]
-    · change (S.cpos _).get _ = (S.cpos _).get _
-      simp only [inv_one, one_smul]
-  mul_smul π₁ π₂ S:= by
-    ext c hc₁ hc₂
-    · change (S.cpos _).Dom ↔ (S.cpos _).Dom
-      simp only [mul_inv_rev, mul_smul]
-    · change (S.cpos _).get _ = (S.cpos _).get _
-      simp only [mul_inv_rev, mul_smul]
-
-
-@[simp]
-theorem smul_mem {ρ : Allowable β} {S : OrdSupport β} {c : SupportCondition β} :
-    c ∈ ρ • S ↔ ρ⁻¹ • c ∈ S :=
-  Iff.rfl
-
-theorem smul_mem_smul {ρ : Allowable β} {S : OrdSupport β} {c : SupportCondition β} :
-    ρ • c ∈ ρ • S ↔ c ∈ S := by
-  simp only [smul_mem, inv_smul_smul]
-
-@[simp]
-theorem smul_cpos {ρ : Allowable β} {S : OrdSupport β} {c : SupportCondition β} :
-    (ρ • S).cpos c = S.cpos (ρ⁻¹ • c) :=
+@[simp, norm_cast]
+theorem coe_sort_coe (S : OrdSupport β) : ((S : Set (SupportCondition β)) : Type _) = S :=
   rfl
 
-theorem smul_cpos_rev {ρ : Allowable β} {S : OrdSupport β} {c : SupportCondition β} :
-    S.cpos (ρ • c) = (ρ⁻¹ • S).cpos c := by
-  simp only [smul_cpos, inv_inv]
+instance : IsWellOrder S S.r := S.r_isWellOrder
 
-theorem smul_cpos_smul {ρ : Allowable β} {S : OrdSupport β} {c : SupportCondition β} :
-    (ρ • S).cpos (ρ • c) = S.cpos c := by
-  simp only [smul_cpos, inv_smul_smul]
+instance : PartialOrder S := partialOrderOfSO S.r
 
-theorem smul_mem_inv {ρ : Allowable β} {S : OrdSupport β} {c : SupportCondition β} :
-    c ∈ ρ⁻¹ • S ↔ ρ • c ∈ S := by
-  simp only [smul_mem, inv_inv]
-
-theorem inv_smul_mem {ρ : Allowable β} {S : OrdSupport β} {c : SupportCondition β} :
-    ρ⁻¹ • c ∈ S ↔ c ∈ ρ • S := by
-  simp only [smul_mem]
-
-theorem smul_eq_of_smul_eq (ρ : Allowable β) {S : OrdSupport β} {c : SupportCondition β}
-    (h : c ∈ S) : ρ • S = S → ρ • c = c := by
-  intro hS
-  have := congr_arg₂ OrdSupport.cpos hS (refl c)
-  refine eq_inv_smul_iff.mp (S.injective c (ρ⁻¹ • c) h ?_ rfl ?_)
-  · rw [← smul_cpos, this]
-    exact h
-  · rw [smul_cpos] at this
-    simp_rw [this]
-
-/-- The restriction of this ordered support to conditions that come before position `i`. -/
-def before (S : OrdSupport β) (i : Atom ⊕ NearLitter) : OrdSupport β where
-  cpos c := ⟨∃ h : c ∈ S, (S.cpos c).get h < i, fun h => (S.cpos c).get h.1⟩
-  injective c d hc hd h := S.injective c d _ _ h
-  dom_small' := by
-    refine Small.mono ?_ S.dom_small
-    intro c hc
-    exact hc.1
-
-@[simp]
-theorem mem_before {S : OrdSupport β} {i : Atom ⊕ NearLitter} (c : SupportCondition β) :
-    c ∈ S.before i ↔ ∃ h : c ∈ S, (S.cpos c).get h < i :=
-  Iff.rfl
-
-@[simp]
-theorem before_get {S : OrdSupport β} {i : Atom ⊕ NearLitter} {c : SupportCondition β}
-    (hc : c ∈ S.before i) :
-    ((S.before i).cpos c).get hc = (S.cpos c).get hc.1 :=
-  rfl
-
-/-- Retains only those support conditions beginning with the path `A`. -/
-def comp (S : OrdSupport β) (γ : Iic α) (A : Quiver.Path (β : TypeIndex) γ) : OrdSupport γ where
-  cpos c := S.cpos ⟨A.comp c.path, c.value⟩
-  injective c d hc hd h₁ h₂ := by
-    have := S.injective _ _ _ _ ?_ h₂
-    · rw [SupportCondition.mk.injEq] at this ⊢
-      rw [Quiver.Path.comp_inj_right] at this
-      exact this
-    · rw [h₁]
-  dom_small' := by
-    change Small ((fun c : SupportCondition γ => ⟨A.comp c.path, c.value⟩) ⁻¹' S.cpos.Dom)
-    refine Small.preimage ?_ S.dom_small
-    intro c d h
-    rw [SupportCondition.mk.injEq] at h ⊢
-    rw [Quiver.Path.comp_inj_right] at h
-    exact h
-
-@[simp]
-theorem mem_comp {S : OrdSupport β} (γ : Iic α) (A : Quiver.Path (β : TypeIndex) γ)
-    (c : SupportCondition γ) :
-    c ∈ S.comp γ A ↔ ⟨A.comp c.path, c.value⟩ ∈ S :=
-  Iff.rfl
-
-@[simp]
-theorem comp_get {S : OrdSupport β} {γ : Iic α} {A : Quiver.Path (β : TypeIndex) γ}
-    {c : SupportCondition γ} (hc : c ∈ S.comp γ A) :
-    ((S.comp γ A).cpos c).get hc = (S.cpos ⟨A.comp c.path, c.value⟩).get hc :=
-  rfl
-
-/-- An ordered support is strong if every element of its domain is reduced, every reduced condition
-it constrains lies in its domain, and the position of each support condition is given by the global
-position function. -/
-structure Strong (S : OrdSupport β) : Prop where
-  reduced_of_mem (c : SupportCondition β) : c ∈ S → Reduced c.value
-  transConstrains_mem (c d : SupportCondition β) : Reduced c.value → c <[α] d → d ∈ S → c ∈ S
-  cpos_get_eq (c : SupportCondition β) (hc : c ∈ S) : (S.cpos c).get hc = c.value
-
-theorem Strong.cpos_eq {S : OrdSupport β} (h : S.Strong) {c : SupportCondition β} :
-    S.cpos c = ⟨c ∈ S, fun _ => c.value⟩ := by
-  refine Part.ext' Iff.rfl ?_
-  intros hc _
-  exact h.cpos_get_eq c hc
-
-theorem Strong.fst_toNearLitter_mem {S : OrdSupport β} (hS : S.Strong)
-    {A : ExtendedIndex β} {a : Atom} (h : ⟨A, inl a⟩ ∈ S) :
-    ⟨A, inr a.1.toNearLitter⟩ ∈ S :=
-  hS.transConstrains_mem _ _
-    (Reduced.mkLitter a.1) (Relation.TransGen.single (Constrains.atom A a)) h
-
-theorem Strong.isLitter_of_mem {S : OrdSupport β} (hS : S.Strong)
-    {A : ExtendedIndex β} {N : NearLitter} (h : ⟨A, inr N⟩ ∈ S) :
-    N.IsLitter := by
-  cases hS.reduced_of_mem _ h
-  exact NearLitter.IsLitter.mk _
-
-def strongSupport (S : Set (SupportCondition β)) (hS : Small S) : OrdSupport β where
-  cpos c := ⟨c ∈ S, fun _ => c.value⟩
-  injective := by intros; ext <;> assumption
-  dom_small' := hS
-
-@[simp]
-theorem strongSupport_cpos (S : Set (SupportCondition β)) (hS : Small S)
-    (c : SupportCondition β) (h : c ∈ S) : ((strongSupport S hS).cpos c).get h = c.value :=
-  rfl
-
-theorem strongSupport_strong (S : Set (SupportCondition β)) (hS : Small S)
-    (hS₁ : ∀ c ∈ S, Reduced c.value) (hS₂ : ∀ c d, Reduced c.value → c <[α] d → d ∈ S → c ∈ S) :
-    (strongSupport S hS).Strong :=
-  ⟨hS₁, hS₂, fun _ _ => rfl⟩
-
-theorem smul_strongSupport_eq (S : Set (SupportCondition β)) (hS : Small S) (ρ : Allowable β)
-    (h : ∀ c ∈ S, ρ • c = c) : ρ • strongSupport S hS = strongSupport S hS := by
-  ext c hcS hcT
-  · simp only [smul_mem]
-    constructor
-    · intro hc
-      have := h _ hc
-      rw [smul_inv_smul] at this
-      rw [this]
-      exact hc
-    · intro hc
-      have := h _ hc
-      rw [← this, inv_smul_smul]
-      exact hc
-  · simp only [smul_cpos, strongSupport_cpos]
-    conv_lhs => rw [← h _ hcT, inv_smul_smul]
-
-/-- `T` *extends* `S` if it is defined wherever `S` is, and agrees with it there, and any
-extra support conditions come after all those in `S`. -/
-structure Extends (T S : OrdSupport β) : Prop where
-  mem_of_mem (c : SupportCondition β) : c ∈ S → c ∈ T
-  get_eq_get (c : SupportCondition β) (hS : c ∈ S) (hT : c ∈ T) :
-    (S.cpos c).get hS = (T.cpos c).get hT
-  /-- If `c` is in `S ∩ T` and `d` is in `T \ S`, then `c` comes before `d`. -/
-  get_lt_get (c d : SupportCondition β) (hcS : c ∈ S) (hcT : c ∈ T) (hdS : d ∉ S) (hdT : d ∈ T) :
-    (T.cpos c).get hcT < (T.cpos d).get hdT
-
-instance : LE (OrdSupport β) where
-  le S T := Extends T S
-
-instance : PartialOrder (OrdSupport β) where
-  le_refl S := by
-    constructor
-    · intro c hc
-      exact hc
-    · intros
-      rfl
-    · intro c d _ _ hdS hdT
-      cases hdS hdT
-  le_trans S T U hST hTU := by
-    constructor
-    · intro c hc
-      exact hTU.mem_of_mem c (hST.mem_of_mem c hc)
-    · intro c hS hU
-      rw [hST.get_eq_get c hS (hST.mem_of_mem c hS), hTU.get_eq_get c (hST.mem_of_mem c hS) hU]
-    · intro c d hcS hcU hdS hdU
-      by_cases hdT : d ∈ T
-      · rw [← hTU.get_eq_get c (hST.mem_of_mem c hcS) hcU, ← hTU.get_eq_get d hdT hdU]
-        exact hST.get_lt_get c d hcS (hST.mem_of_mem c hcS) hdS hdT
-      · exact hTU.get_lt_get c d (hST.mem_of_mem c hcS) hcU hdT hdU
-  le_antisymm S T hST hTS := by
-    ext c hS hT
-    · constructor
-      · exact hST.mem_of_mem c
-      · exact hTS.mem_of_mem c
-    · exact hST.get_eq_get c hS hT
-
-theorem smul_le_smul {S T : OrdSupport β} (h : S ≤ T) (ρ : Allowable β) : ρ • S ≤ ρ • T := by
-  constructor
-  · intro c
-    exact h.mem_of_mem (ρ⁻¹ • c)
-  · intro c
-    exact h.get_eq_get (ρ⁻¹ • c)
-  · intro c d
-    exact h.get_lt_get (ρ⁻¹ • c) (ρ⁻¹ • d)
-
-theorem smul_le_iff_le_inv {S T : OrdSupport β} (ρ : Allowable β) : S ≤ ρ⁻¹ • T ↔ ρ • S ≤ T := by
-  constructor
-  · intro h
-    have := smul_le_smul h ρ
-    rw [smul_inv_smul] at this
-    exact this
-  · intro h
-    have := smul_le_smul h ρ⁻¹
-    rw [inv_smul_smul] at this
-    exact this
+open scoped Classical in
+noncomputable instance : LinearOrder S := linearOrderOfSTO S.r
 
 end OrdSupport
 
