ConNF/Counting.lean
@@ -1,11 +1,1 @@
 import ConNF.Counting.OrdSupport
-import ConNF.Counting.Reorder
-import ConNF.Counting.OrdSupportEquiv
-import ConNF.Counting.CodingFunction
-import ConNF.Counting.CodingFunctionEquiv
-import ConNF.Counting.Spec
-import ConNF.Counting.SpecSame
-import ConNF.Counting.OrdSupportExtend
-import ConNF.Counting.OrdSupportOrbit
-import ConNF.Counting.Recode
-import ConNF.Counting.CountTangles
